exercises/project02-sharded-kv-store/RefinementProof.v.dfy
@@ -27,15 +27,19 @@ module RefinementProof refines RefinementObligation {
         // What does it mean for host id to own a key (and assign it the value
         // val)?
         // FIXME: fill in here (solution: 3 lines)
-        true
+        && v.ValidHost(id)
+        && k in v.hosts[id].m
+        && v.hosts[id].m[k] == val
       // END EDIT
       case MessageOwner(msg) =>
         // What does it mean for the network to own a key (and assign it the
         // value val)? This is a new concept relative to the atomic demo from
         // chapter06.
         // FIXME: fill in here (solution: 3 lines)
-        true
-        // END EDIT
+        && msg in v.network.inFlightMessages
+        && msg.key == k
+        && msg.value == val
+           // END EDIT
     }
   }
 
@@ -45,6 +49,7 @@ module RefinementProof refines RefinementObligation {
     && IsFull(av.table)
        // Use OwnerValue to connect v to av
        // FIXME: fill in here (solution: 1 line)
+    && (forall k, val | (exists o :: OwnerValue(v, o, k, val)) :: av.table[k] == val)
        // END EDIT
   }
 
@@ -139,8 +144,10 @@ module RefinementProof refines RefinementObligation {
   ghost predicate Inv(v: Variables)
   {
     // FIXME: fill in here (solution: 3 lines)
-    true
-    // END EDIT
+    && v.WF()
+    && (forall k | IsKey(k) :: OwnersDistinct(v, k))
+    && (exists owners :: OwnerHasSomeValue(v, owners))
+       // END EDIT
   }
 
   ////////////////////////////////////////////////////////////////////////////
@@ -152,6 +159,24 @@ module RefinementProof refines RefinementObligation {
     ensures AtomicKV.Init(VariablesAbstraction(v))
   {
     // FIXME: fill in here (solution: 12 lines)
+    assert forall k | IsKey(k) :: OwnersDistinct(v, k) by {
+      reveal OwnersDistinct();
+    }
+
+    var owners := imap k | IsKey(k) :: HostOwner(0);
+    assert OwnerHasSomeValue(v, owners) by {
+      assert forall k | IsKey(k) :: OwnerValue(v, HostOwner(0), k, 0);
+      reveal OwnerHasSomeValue();
+    }
+
+    var av := VariablesAbstraction(v);
+    assert AtomicKV.Init(av) by {
+      assert AbstractionRelation(v, AtomicKV.Variables(table := ZeroMap()));
+      forall k | IsKey(k) ensures av.table[k] == 0 {
+        assert OwnerValue(v, HostOwner(0), k, 0);
+      }
+      imap_ext_eq(av.table, ZeroMap());
+    }
     // END EDIT
   }
 
@@ -159,6 +184,212 @@ module RefinementProof refines RefinementObligation {
   // Your proof goes here. We highly, highly recommend stating and proving a
   // refinement lemma for each step; see the chapter06 demo if you need help
   // structuring that.
+  lemma OpPreservesOwnerHasSomeValue(v: Variables, v': Variables, id: HostId, msgOps: Network.MessageOps, event: Event, step: Host.Step)
+    requires Inv(v)
+    requires Next(v, v', event)
+    requires v.ValidHost(id)
+    requires Host.NextStep(v.hosts[id], v'.hosts[id], msgOps, event, step)
+    requires exists dsstep :: NextStep(v, v', event, dsstep) && msgOps == dsstep.msgOps
+    ensures exists owners :: OwnerHasSomeValue(v', owners)
+  {
+    var owner := if step.SendStep? then MessageOwner(msgOps.send.value) else HostOwner(id);
+    var oldOwners :| OwnerHasSomeValue(v, oldOwners);
+    var newOwners := oldOwners[step.key := owner];
+    assert OwnerHasSomeValue(v', newOwners) by {
+      forall k | IsKey(k) ensures exists val :: OwnerValue(v', newOwners[k], k, val) {
+        if (k == step.key) {
+          assert OwnerValue(v', owner, k, step.value);
+        } else {
+          var oldVal := use_OwnerHasSomeValue(v, oldOwners, k);
+          assert OwnerValue(v', newOwners[k], k, oldVal);
+        }
+      }
+      reveal OwnerHasSomeValue();
+    }
+  }
+
+  lemma OpPerservesOwnersDistinctForOtherKeys(v: Variables, v': Variables, id: HostId, msgOps: Network.MessageOps, event: Event, step: Host.Step)
+    requires Inv(v)
+    requires Next(v, v', event)
+    requires v.ValidHost(id)
+    requires Host.NextStep(v.hosts[id], v'.hosts[id], msgOps, event, step)
+    requires exists dsstep :: NextStep(v, v', event, dsstep) && msgOps == dsstep.msgOps
+    ensures forall k | k != step.key :: OwnersDistinct(v', k)
+  {
+    forall k | k != step.key ensures OwnersDistinct(v', k) {
+      forall o1: MapOwner, o2: MapOwner, val1: int, val2: int
+        | OwnerValue(v', o1, k, val1) && OwnerValue(v', o2, k, val2)
+        ensures o1 == o2 && val1 == val2 {
+        use_OwnersDistinct(v, k, o1, val1, o2, val2);
+      }
+      reveal OwnersDistinct();
+    }
+  }
+
+  ghost function GetValue(v: Variables, k: int) : int
+    requires Inv(v)
+  {
+    reveal OwnerHasSomeValue();
+    var val :| exists owner :: OwnerValue(v, owner, k, val);
+    val
+  }
+
+  lemma InvImpliesFull(v: Variables)
+    requires Inv(v)
+    ensures IsFull(VariablesAbstraction(v).table)
+  {
+    reveal OwnersDistinct();
+
+    var av := AtomicKV.Variables(table := imap k :: GetValue(v, k));
+    forall k, val, o | OwnerValue(v, o, k, val) ensures av.table[k] == val {
+      var owners : Owners :| OwnerHasSomeValue(v, owners);
+      use_OwnerValue(v, owners, o, k, val);
+    }
+    assert AbstractionRelation(v, av);
+  }
+
+  lemma OpPerservesValueForOtherKeys(v: Variables, v': Variables, id: HostId, msgOps: Network.MessageOps, event: Event, step: Host.Step)
+    requires Inv(v) && Inv(v')
+    requires Next(v, v', event)
+    requires v.ValidHost(id)
+    requires Host.NextStep(v.hosts[id], v'.hosts[id], msgOps, event, step)
+    requires exists dsstep :: NextStep(v, v', event, dsstep) && msgOps == dsstep.msgOps
+    ensures IsFull(VariablesAbstraction(v).table)
+    ensures IsFull(VariablesAbstraction(v').table)
+    ensures forall k | k != step.key :: VariablesAbstraction(v).table[k] == VariablesAbstraction(v').table[k]
+  {
+    InvImpliesFull(v);
+    InvImpliesFull(v');
+
+    var av := VariablesAbstraction(v);
+    var av' := VariablesAbstraction(v');
+    forall k | k in av.table + av'.table && k != step.key ensures av.table[k] == av'.table[k] {
+      var owners : Owners :| OwnerHasSomeValue(v, owners);
+      var val := use_OwnerHasSomeValue(v, owners, k);
+      assert OwnerValue(v', owners[k], k, val);
+    }
+  }
+
+  lemma GetPreservesInvAndRefines(v: Variables, v': Variables, id: HostId, msgOps: Network.MessageOps, event: Event, step: Host.Step)
+    requires Inv(v)
+    requires Next(v, v', event)
+    requires v.ValidHost(id)
+    requires Host.NextStep(v.hosts[id], v'.hosts[id], msgOps, event, step)
+    requires step.GetStep?
+    ensures Inv(v')
+    ensures AtomicKV.Next(VariablesAbstraction(v), VariablesAbstraction(v'), event)
+  {
+    assert v == v';
+    OpPerservesValueForOtherKeys(v, v', id, msgOps, event, step);
+    assert OwnerValue(v, HostOwner(id), step.key, step.value);
+  }
+
+  lemma PutPreservesInvAndRefines(v: Variables, v': Variables, id: HostId, msgOps: Network.MessageOps, event: Event, step: Host.Step)
+    requires Inv(v)
+    requires Next(v, v', event)
+    requires v.ValidHost(id)
+    requires Host.NextStep(v.hosts[id], v'.hosts[id], msgOps, event, step)
+    requires step.PutStep?
+    ensures Inv(v')
+    ensures AtomicKV.Next(VariablesAbstraction(v), VariablesAbstraction(v'), event)
+  {
+    OpPerservesOwnersDistinctForOtherKeys(v, v', id, msgOps, event, step);
+    OpPreservesOwnerHasSomeValue(v, v', id, msgOps, event, step);
+
+    assert OwnersDistinct(v', step.key) by {
+      forall o: MapOwner, val: int | OwnerValue(v', o, step.key, val)
+        ensures o == HostOwner(id) && val == step.value {
+        match o {
+          case MessageOwner(msg') =>
+            use_OwnersDistinct(v, step.key, HostOwner(id), v.hosts[id].m[step.key], MessageOwner(msg'), msg'.value);
+            assert false;
+          case HostOwner(id') =>
+            use_OwnersDistinct(v, step.key, HostOwner(id), v.hosts[id].m[step.key], HostOwner(id'), v.hosts[id'].m[step.key]);
+        }
+      }
+      reveal OwnersDistinct();
+    }
+
+    assert AtomicKV.Next(VariablesAbstraction(v), VariablesAbstraction(v'), event) by {
+      OpPerservesValueForOtherKeys(v, v', id, msgOps, event, step);
+      assert OwnerValue(v', HostOwner(id), step.key, step.value);
+    }
+  }
+
+  lemma SendPreservesInvAndRefines(v: Variables, v': Variables, id: HostId, msgOps: Network.MessageOps, event: Event, step: Host.Step)
+    requires Inv(v)
+    requires Next(v, v', event)
+    requires v.ValidHost(id)
+    requires Host.NextStep(v.hosts[id], v'.hosts[id], msgOps, event, step)
+    requires exists dsstep :: NextStep(v, v', event, dsstep) && msgOps == dsstep.msgOps
+    requires step.SendStep?
+    ensures Inv(v')
+    ensures AtomicKV.Next(VariablesAbstraction(v), VariablesAbstraction(v'), event)
+  {
+    OpPerservesOwnersDistinctForOtherKeys(v, v', id, msgOps, event, step);
+    OpPreservesOwnerHasSomeValue(v, v', id, msgOps, event, step);
+
+    assert OwnersDistinct(v', step.key) by {
+      forall o: MapOwner, val: int | OwnerValue(v', o, step.key, val)
+        ensures o == MessageOwner(msgOps.send.value) && val == step.value {
+        match o {
+          case MessageOwner(msg') =>
+            if (msg'.value != step.value) {
+              use_OwnersDistinct(v, step.key, HostOwner(id), v.hosts[id].m[step.key], MessageOwner(msg'), msg'.value);
+              assert false;
+            }
+          case HostOwner(id') =>
+            use_OwnersDistinct(v, step.key, HostOwner(id), v.hosts[id].m[step.key], HostOwner(id'), v.hosts[id'].m[step.key]);
+            assert false;
+        }
+      }
+      reveal OwnersDistinct();
+    }
+
+    assert AtomicKV.Next(VariablesAbstraction(v), VariablesAbstraction(v'), event) by {
+      OpPerservesValueForOtherKeys(v, v', id, msgOps, event, step);
+      assert OwnerValue(v, HostOwner(id), step.key, step.value);
+      assert OwnerValue(v', MessageOwner(msgOps.send.value), step.key, step.value);
+    }
+  }
+
+  lemma RecvPreservesInvAndRefines(v: Variables, v': Variables, id: HostId, msgOps: Network.MessageOps, event: Event, step: Host.Step)
+    requires Inv(v)
+    requires Next(v, v', event)
+    requires v.ValidHost(id)
+    requires Host.NextStep(v.hosts[id], v'.hosts[id], msgOps, event, step)
+    requires exists dsstep :: NextStep(v, v', event, dsstep) && msgOps == dsstep.msgOps
+    requires step.RecvStep?
+    ensures Inv(v')
+    ensures AtomicKV.Next(VariablesAbstraction(v), VariablesAbstraction(v'), event)
+  {
+    OpPerservesOwnersDistinctForOtherKeys(v, v', id, msgOps, event, step);
+    OpPreservesOwnerHasSomeValue(v, v', id, msgOps, event, step);
+
+    assert OwnersDistinct(v', step.key) by {
+      forall o: MapOwner, val: int | OwnerValue(v', o, step.key, val)
+        ensures o == HostOwner(id) && val == step.value {
+        var msg := msgOps.recv.value;
+        match o {
+          case MessageOwner(msg') =>
+            use_OwnersDistinct(v, step.key, MessageOwner(msg), msg.value, MessageOwner(msg'), msg'.value);
+            assert false;
+          case HostOwner(id') =>
+            if (id' != id) {
+              use_OwnersDistinct(v, step.key, MessageOwner(msg), msg.value, HostOwner(id'), v.hosts[id'].m[step.key]);
+              assert false;
+            }
+        }
+      }
+      reveal OwnersDistinct();
+    }
+
+    assert AtomicKV.Next(VariablesAbstraction(v), VariablesAbstraction(v'), event) by {
+      OpPerservesValueForOtherKeys(v, v', id, msgOps, event, step);
+      assert OwnerValue(v, MessageOwner(msgOps.recv.value), step.key, step.value);
+      assert OwnerValue(v', HostOwner(id), step.key, step.value);
+    }
+  }
   // END EDIT
 
   lemma RefinementNext(v: Variables, v': Variables, event: Event)
@@ -177,6 +408,16 @@ module RefinementProof refines RefinementObligation {
     // All the solution dos here is match on the step and call the lemma for
     // refinement of that step.
     // FIXME: fill in here (solution: 14 lines)
+    match step {
+      case GetStep(key, value) =>
+        GetPreservesInvAndRefines(v, v', id, msgOps, event, step);
+      case PutStep(key, value) =>
+        PutPreservesInvAndRefines(v, v', id, msgOps, event, step);
+      case SendStep(key, value) =>
+        SendPreservesInvAndRefines(v, v', id, msgOps, event, step);
+      case RecvStep(key, value) =>
+        RecvPreservesInvAndRefines(v, v', id, msgOps, event, step);
+    }
     // END EDIT
   }
 }
